stlc bred with dep typed syntax

lib/Stlc.v
@@ -1,4 +1,4 @@
-Require Import Lambda.Util Coq.Program.Equality.
+Require Export Lambda.SimpleTypes.
 
 (** Note: many of the helper lemmas
           and proof techniques
@@ -8,17 +8,6 @@ Require Import Lambda.Util Coq.Program.Equality.
 *)
 
 (** * De Bruijn Syntax *)
-
-Inductive type : Set :=
-| Base
-| Arrow (t1 t2 : type).
-(**[]*)
-
-Declare Scope ty_scope.
-Delimit Scope ty_scope with ty.
-Notation "⊥" := Base (at level 0) : ty_scope.
-Notation "t1 '→' t2" := (Arrow t1 t2) (at level 5, right associativity) : ty_scope.
-Open Scope ty_scope.
 
 Inductive expr : Set :=
 | Var (n : nat)
@@ -88,10 +77,6 @@ Fixpoint shift (c i : nat) (e : expr) : expr :=
   | e1 ⋅ e2 => (shift c i e1) ⋅ (shift c i e2)
   end.
 (**[]*)
-
-Ltac destroy_arith :=
-  intros; simpl; clean_compare;
-  try (f_equal; auto 2; lia).
 
 Section ShiftLemmas.
   Lemma shift0 : forall e k, shift k 0 e = e.
@@ -531,55 +516,7 @@ Section SNProp.
   Qed.
 End SNProp.
 
-Module StrongNorm.  
-  Fixpoint teqb (t1 t2 : type) : bool :=
-    match t1, t2 with
-    | ⊥, ⊥ => true
-    | T1 → t1, T2 → t2 => teqb T1 T2 && teqb t1 t2
-    | _, _ => false
-    end.
-  (**[]*)
-
-  Section TypeEq.
-    Local Hint Resolve andb_true_intro : core.
-    
-    Lemma teqb_refl : forall t, teqb t t = true.
-    Proof.
-      intro t; induction t; simpl; intuition.
-    Qed.
-
-    Hint Rewrite Bool.andb_true_iff : core.
-
-    Lemma eq_teqb : forall t1 t2, teqb t1 t2 = true -> t1 = t2.
-    Proof.
-      intro t1; induction t1; intros []; simpl;
-        autorewrite with core; intuition;
-          f_equal; eauto.
-    Qed.
-
-    Local Hint Resolve eq_teqb : core.
-    Local Hint Resolve teqb_refl : core.
-    Hint Rewrite teqb_refl : core.
-
-    Lemma teqb_eq : forall t1 t2, teqb t1 t2 = true <-> t1 = t2.
-    Proof.
-      intuition; subst; trivial.
-    Qed.
-
-    Local Hint Resolve teqb_eq : core.
-    Hint Rewrite teqb_eq : core.
-    Local Hint Constructors Bool.reflect : core.
-
-    Lemma teqb_reflect : forall t1 t2,
-        Bool.reflect (t1 = t2) (teqb t1 t2).
-    Proof.
-      intros t1 t2.
-      destruct (teqb t1 t2) eqn:Hteqb; auto.
-      constructor. intros H.
-      apply teqb_eq in H.
-      rewrite H in Hteqb. discriminate.
-    Qed.
-  End TypeEq.
+Module StrongNorm.
 
   Fixpoint types (g : list type) (e : expr) : option type :=
     match e with
