lib/StlcDep.v
@@ -1,4 +1,4 @@
-From Lambda Require Export Util Stlc.
+Require Export Lambda.SimpleTypes.
 
 (** * Dependently Typed Lambda Calculus. *)
 
@@ -9,6 +9,12 @@ From Lambda Require Export Util Stlc.
 
 Section List.
   Context {A : Set}.
+
+  Fixpoint Has (a : A) (Γ : list A) : Set :=
+    match Γ with
+    | []    => Empty_set
+    | h :: Δ => ((h = a) + Has a Δ)%type
+    end.
 
   Definition lookup :
     forall {Γ : list A} {n : nat},
@@ -71,33 +77,220 @@ Section List.
       intros [| n] H; cbn in *;
         try lia; eauto using Lt.lt_S_n.
   Defined.
+
+  Definition ext' : forall {Γ Δ},
+      (forall a, Has a Γ -> Has a Δ) ->
+      forall b a, Has a (b :: Γ) -> Has a (b :: Δ).
+  Proof.
+    refine
+      (fun l d f b a H =>
+         match l as l' return l = l' -> Has a (b :: d) with
+         | [] => fun Hl => inl _
+         | h :: t
+           => fun Hl =>
+               match H with
+               | inl Hh => inl Hh
+               | inr Ht => inr (f _ Ht)
+               end
+         end eq_refl); subst; cbn in *.
+    destruct H as [H | H]; subst; reflexivity || contradiction.
+  Defined.
+
+  Definition Has_nth_error : forall {Γ a},
+      Has a Γ -> { n | nth_error Γ n = Some a}.
+  Proof.
+    intro l; induction l as [| h t IHt];
+      intros a Hal; cbn in *; try contradiction.
+    destruct Hal as [Hha | Hat]; subst.
+    - refine (exist _ 0 _); reflexivity.
+    - apply IHt in Hat as [k Hk].
+      refine (exist _ (S k) _); assumption.
+  Defined.
+
+  Definition nth_error_Has : forall {Γ a n},
+      nth_error Γ n = Some a -> Has a Γ.
+  Proof.
+    intro l; induction l as [| h t IHt];
+      intros a [| n] Hnth; cbn in *; try discriminate.
+    - inv Hnth; left; reflexivity.
+    - apply IHt in Hnth; right; assumption.
+  Defined.
+
+  Definition nth_error_Has' : forall {Γ a},
+      {n | nth_error Γ n = Some a} -> Has a Γ.
+  Proof.
+    intros l a [n H]; exact (nth_error_Has H).
+  Defined.
+
+  Fail Definition nth_error_Has : forall {Γ a},
+      Has a Γ <-> {n | nth_error Γ n = Some a}.
+  
+  Definition ext : forall {Γ Δ : list A},
+      (forall a, {n | nth_error Γ n = Some a} ->
+              {k | nth_error Δ k = Some a}) ->
+      forall b a, {n | nth_error (b :: Γ) n = Some a} ->
+               {k | nth_error (b :: Δ) k = Some a}.
+  Proof.
+    intros l d f b a Hab.
+    apply Has_nth_error.
+    apply nth_error_Has' in Hab.
+    pose proof (fun a H => nth_error_Has' (f a (Has_nth_error H))) as H.
+    eauto using ext'.
+  Defined.
 End List.
 
 (** De Bruijn syntax. *)
 
-Reserved Notation "Γ '⊩' τ" (at level 80, no associativity).
+Declare Scope term_scope.
+Delimit Scope term_scope with term.
+
+Reserved Notation "Γ '⊢' τ" (at level 80, no associativity).
 
 Inductive term (Γ : list type) : type -> Set :=
 | Id (n : nat) (τ : type) :
     nth_error Γ n = Some τ ->
-    Γ ⊩ τ
+    Γ ⊢ τ
 | Abs (τ τ' : type) :
-    τ :: Γ ⊩ τ' ->
-    Γ ⊩ τ → τ'
+    τ :: Γ ⊢ τ' ->
+    Γ ⊢ τ → τ'
 | App (τ τ' : type) :
-    Γ ⊩ τ → τ' ->
-    Γ ⊩ τ ->
-    Γ ⊩ τ'
-where "Γ '⊩' τ" := (term Γ τ).
+    Γ ⊢ τ → τ' ->
+    Γ ⊢ τ ->
+    Γ ⊢ τ'
+where "Γ '⊢' τ" := (term Γ τ) : term_scope.
 
 Local Hint Constructors term : core.
 
 Definition term_of_id :
-  forall {Γ : list type} (n : nat) {H : n < length Γ},
-    Γ ⊩ lookup H := ltac:(eauto using nth_error_lookup).
+  forall {Γ : list type} (n : nat) (H : n < length Γ),
+    (Γ ⊢ lookup H)%term := ltac:(eauto using nth_error_lookup).
 
+Definition term_of_nth_error
+           {Γ τ} (H : {n | nth_error Γ n = Some τ})
+  : (Γ ⊢ τ)%term :=
+  match H with
+  | exist _ _ Hn => Id _ _ _ Hn
+  end.
+
+Definition App_eq
+           (Γ : list type) (τ ρ σ : type)
+           (t₁ : (Γ ⊢ τ → ρ)%term) (t₂ : (Γ ⊢ σ)%term)
+  : τ = σ -> (Γ ⊢ ρ)%term.
+Proof.
+  intros H; subst; exact (App _ _ _ t₁ t₂).
+Defined.
+
+Local Hint Resolve App_eq : core.
+
+Definition App_lookup
+           (Γ : list type) (n : nat) (H : n < length Γ) (τ ρ : type)
+           (t₁ : (Γ ⊢ lookup H)%term) (t₂ : (Γ ⊢ τ)%term) :
+  lookup H = τ → ρ -> (Γ ⊢ ρ)%term.
+Proof.
+  intros Heq; rewrite Heq in t₁; eauto using App.
+Defined.
+
+Local Hint Resolve App_lookup : core.
+
+Notation "'ID' x"
+  := (Id _ x _)
+       (at level 10, no associativity) : term_scope.
+Notation "'`λ' t"
+  := (Abs _ _ _ t)
+       (at level 15, right associativity) : term_scope.
+Notation "'λ' τ '⇒' t"
+  := (Abs _ τ _ t)
+       (at level 15, right associativity) : term_scope.
+Notation "'λ' τ '↣' .. '↣' ρ '⇒' t"
+  := (Abs _ τ _ .. (Abs _ ρ _ t) ..)
+       (at level 15, right associativity) : term_scope.
+Notation "x '⋅' y"
+  := (App _ _ _ x y)
+       (at level 14, left associativity) : term_scope.
+
+Set Warnings "-non-reversible-notation".
 Notation "'#' n"
-  := (ltac:(refine (term_of_id n); cbn; lia))
-       (at level 10, no associativity).
+  := (ltac:(refine (term_of_id n _); cbn; lia))
+       (at level 10, no associativity) : term_scope.
+Notation "∫ t"
+  := (ltac:(refine (Abs _ _ _ _ t); cbn; eauto))
+       (at level 15, right associativity) : term_scope.
+Notation "x '`⋅' y"
+  := (ltac:(refine (App _ _ _ x y); reflexivity))
+       (at level 14, left associativity) : term_scope.
+Set Warnings "non-reversible-notation".
 
-Example identity_func : [] ⊩ (⊥ → ⊥) := Abs _ _ _ (# 0).
+Fixpoint Rename
+         {Γ Δ}
+         (f: forall τ, {n | nth_error Γ n = Some τ} ->
+                  {k | nth_error Δ k = Some τ})
+         {σ} (t: (Γ ⊢ σ)%term) : (Δ ⊢ σ)%term :=
+  match t with
+  | Id _ _ _ Hm     => term_of_nth_error (f _ (exist _ _ Hm))
+  | Abs _ ρ _ t'    => (`λ Rename (ext f ρ) t')%term
+  | App _ _ _ t₁ t₂ => (Rename f t₁ ⋅ Rename f t₂)%term
+  end.
+
+Definition exts' : forall {Γ Δ},
+    (forall τ, Has τ Γ -> (Δ ⊢ τ)%term) ->
+    forall {ρ σ}, Has σ (ρ :: Γ) -> (ρ :: Δ ⊢ σ)%term.
+Proof.
+  cbn; intros Γ Δ f ρ σ [H | H]; subst.
+  - refine (Id _ 0 _ _); reflexivity.
+  - refine (Rename _ (f _ H)).
+    intros τ Hτ.
+    apply nth_error_Has' in Hτ.
+    apply Has_nth_error; cbn.
+    right; assumption.
+Defined.
+
+Definition exts : forall {Γ Δ},
+    (forall τ, {n | nth_error Γ n = Some τ} -> (Δ ⊢ τ)%term) ->
+    forall ρ σ, {k | nth_error (ρ :: Γ) k = Some σ} -> (ρ :: Δ ⊢ σ)%term.
+Proof.
+  intros Γ Δ f ρ σ H.
+  apply nth_error_Has' in H.
+  pose proof (fun t H => f t (Has_nth_error H)) as f'.
+  exact (exts' f' H).
+Defined.
+
+Fixpoint subs
+         {Γ Δ}
+         (f : forall τ, {n | nth_error Γ n = Some τ} -> (Δ ⊢ τ)%term)
+         {σ} (t : (Γ ⊢ σ)%term) : (Δ ⊢ σ)%term :=
+  match t with
+  | Id _ _ _ Hn => f _ (exist _ _ Hn)
+  | Abs _ ρ _ t' => (`λ subs (exts f ρ) t')%term
+  | App _ _ _ t₁ t₂ => (subs f t₁ ⋅ subs f t₂)%term
+  end.
+
+Definition sub
+           {Γ τ σ}
+           (body : (τ :: Γ ⊢ σ)%term) (arg : (Γ ⊢ τ)%term)
+  : (Γ ⊢ σ)%term.
+Proof.
+  refine (subs _ body).
+  intros ρ [n Hρ].
+  destruct n as [| n]; cbn in *.
+  - inv Hρ. apply arg.
+  - eauto using term_of_nth_error.
+Defined.
+
+Notation "x '[[' y ']]'"
+  := (sub x y) (at level 12, no associativity) : term_scope.
+
+Reserved Notation "x '-->' y" (at level 80, no associativity).
+
+Inductive bred {Γ} : forall {τ}, (Γ ⊢ τ)%term -> (Γ ⊢ τ)%term -> Prop :=
+| bred_bred τ τ' (t₁ : (τ :: Γ ⊢ τ')%term) t₂ :
+    ((`λ t₁) ⋅ t₂)%term --> (t₁ [[ t₂ ]])%term
+| bred_abs τ τ' (t t' : (τ :: Γ ⊢ τ')%term) :
+    t -->  t' ->
+    (`λ t)%term --> (`λ t')%term
+| bred_app_l τ τ' (t₁ t₁' : (Γ ⊢ τ → τ')%term) t₂ :
+    t₁ -->  t₁' ->
+    (t₁ ⋅ t₂)%term -->  (t₁' ⋅ t₂)%term
+| bred_app_r τ τ' (t₁ : (Γ ⊢ τ → τ')%term) t₂ t₂' :
+    t₂ -->  t₂' ->
+    (t₁ ⋅ t₂)%term -->  (t₁ ⋅ t₂')%term
+where "x '-->' y" := (bred x y) : type_scope.
