lib/StlcDepExamples.v
@@ -1,0 +1,34 @@
+Require Export Lambda.StlcDep.
+
+Module Examples.
+  Open Scope term_scope.
+  
+  Example _identity_func : [] ⊢ ⊥ → ⊥ := λ ⊥ ⇒ # 0.
+  Compute _identity_func.
+
+  Example _nat : type := (⊥ → ⊥) → ⊥ → ⊥.
+  Local Hint Unfold _nat : core.
+
+  Example _zero : [] ⊢ _nat := λ ⊥ → ⊥ ⇒ λ ⊥ ⇒ # 0.
+  Example _zero' : [] ⊢ _nat := `λ `λ # 0.
+  Example _zero'' : [] ⊢ _nat := λ ⊥ → ⊥ ↣ ⊥ ⇒ # 0.
+
+  Example _one : [] ⊢ _nat.
+  Proof.
+    refine (λ ⊥ → ⊥ ↣ ⊥ ⇒ ID 1 _ ⋅ ID 0 _); reflexivity.
+  Defined.
+
+  Fail Example _one' : [] ⊢ _nat := ∫ ∫ ID 1 _ `⋅ ID 0 _.
+
+  Example _succ : [] ⊢ _nat → _nat.
+  Proof.
+    refine (λ _nat ⇒ λ ⊥ → ⊥ ↣ ⊥ ⇒ ID 1 _ ⋅ (ID 2 _ ⋅ ID 1 _ ⋅ ID 0 _)); reflexivity.
+  Defined.
+
+  Example _two : [] ⊢ _nat.
+  Proof.
+    refine (`λ `λ ID 1 _ ⋅ (ID 1 _ ⋅ ID 0 _)); reflexivity.
+  Defined.
+
+  Compute _succ ⋅ _zero.
+End Examples.
